WHILE takes a machine parametrised over (option F) instead of (bool*F).
TODO: adjust all machines using WHILE

TM/Combinators/While.v
@@ -10,19 +10,35 @@ Section While.
   Variable sig : finType.
 
   Variable F : finType.
-  Variable pM : { M : mTM sig n & states M -> bool * F }.
+  (** Parameter [None] indicates continueing, [Some f] means breaking out of the loop and terminating in the partition [f]. *)
+  Variable pM : { M : mTM sig n & states M -> option F }.
 
   Definition while_trans :
     (TM.states (projT1 pM)) * Vector.t (option sig) n ->
     (TM.states (projT1 pM)) * Vector.t (option sig * move) n :=
-    fun st => let (s,a) := st in
-           if fst (projT2 pM s) && halt s then (start (projT1 pM),null_action) else trans st.
+    fun '(s,t) =>
+      if halt s
+      then match projT2 pM s with
+           | Some y => trans (s,t)
+           | None => (start (projT1 pM), null_action)
+           end
+      else trans (s,t).
 
   Definition While : mTM sig n :=
     Build_mTM while_trans (start (projT1 pM))
-              (fun s => halt s && negb (fst (projT2 pM s))).
+              (fun s => halt s && match projT2 pM s with
+                               | Some _ => true
+                               | None => false
+                               end).
 
-  Definition WHILE := (While; fun s => snd (projT2 pM s)).
+  Hypothesis (defF : inhabitedC F).
+
+  Definition WHILE : pTM sig F n :=
+    (While; fun s =>
+              match projT2 pM s with
+              | Some y => y
+              | None => default
+              end).
 
   Local Arguments loopM {_ _} _ _ _.
   Local Arguments halt {_ _} _ _.
@@ -33,7 +49,7 @@ Section While.
   Proof.
     intros s. exact (if (halt (projT1 pM) (cstate s)) then Some s else None).
   Defined.
- 
+
   Lemma While_split i res c:
     loopM While i c = Some res ->
     exists i1 x1 i2,
@@ -48,12 +64,12 @@ Section While.
       eapply loop_lift with (lift:=id) in H1.
       + exact H1.
       + reflexivity.
-      + unfold id.  intros. destruct x. unfold step. cbn in *. rewrite H. now rewrite andb_false_r.
-    - intros b. unfold halt at 2. cbn. now intros ->. 
+      + unfold id.  intros. destruct x. unfold step. cbn in *. now rewrite H.
+    - intros b. unfold halt at 2. cbn. now intros ->.
   Qed.
 
-  Lemma While_true_split i (x : mconfig _ (states While) _) oenc (f : F) :
-    halt (projT1 pM) (cstate x) = true  -> projT2 pM (cstate x) = (true, f) ->
+  Lemma While_true_split i (x : mconfig _ (states While) _) oenc :
+    halt (projT1 pM) (cstate x) = true -> projT2 pM (cstate x) = None ->
     loopM While i x = Some oenc ->
     exists i', i = 1+i' /\ loopM While i' (initc While (ctapes x)) = Some oenc.
   Proof.
@@ -61,14 +77,14 @@ Section While.
     destruct i as [ |i'];cbn in Eq;cbn in Eq; change (states (projT1 pM)) with (states While) in Eq; rewrite hx,px in Eq;cbn in Eq; inv Eq.
     exists i'. split;[omega| ].
     destruct x. cbn in *. rewrite <- H0. unfold loopM. f_equal.
-    unfold step. cbn -[tape_move_multi null_action]. 
+    unfold step. cbn -[tape_move_multi null_action].
     rewrite hx,px. cbn -[tape_move_multi null_action]. now rewrite tape_move_null_action.
   Qed.
 
-  Lemma While_true_merge i1 i2 (t x1 : mconfig _ (states While) _) oenc (f : F) :
+  Lemma While_true_merge i1 i2 (t x1 : mconfig _ (states While) _) oenc :
     loopM (projT1 pM) i1 t = Some x1 ->
     loopM While i2 (initc While (ctapes x1)) = Some oenc ->
-    (projT2 pM) (cstate x1) = (true, f) ->
+    (projT2 pM) (cstate x1) = None ->
     loopM While (i1+(1+i2)) t = Some oenc.
   Proof.
     intros Eq1 Eq2 px1.
@@ -77,18 +93,18 @@ Section While.
     {unfold While. cbn. intros. now destruct halt. }
     {change (states While) with (states (projT1 pM)) in *.
      eapply loop_lift with (g:= step While) in Eq1;[exact Eq1|reflexivity| ].
-     intros. unfold step,While,while_trans. cbn. now rewrite H,andb_false_r.
+     intros. unfold step,While,while_trans. cbn. now rewrite H.
     }
     cbn. assert (hx1:halt (projT1 pM) (cstate x1)=true) by (apply loop_fulfills_p in Eq1;now destruct halt).
     change (states While) with (states (projT1 pM)) in *.
     rewrite hx1;cbn.
     -rewrite <- Eq2. unfold loopM. cbn. f_equal. unfold step. cbn -[tape_move_multi null_action].
-     rewrite hx1,px1;cbn -[tape_move_multi null_action]. now rewrite tape_move_null_action. 
+     rewrite hx1,px1;cbn -[tape_move_multi null_action]. now rewrite tape_move_null_action.
   Qed.
 
    Lemma While_false_merge i1 (t : mconfig _ (states While) _) oenc (f : F) :
     loopM (projT1 pM) i1 t = Some oenc ->
-    projT2 pM (cstate oenc) = (false, f) ->
+    projT2 pM (cstate oenc) = Some f ->
     loopM While i1 t = Some oenc.
   Proof.
     intros Eq px1.
@@ -96,21 +112,22 @@ Section While.
       in Eq. destruct Eq as (?&H'&H1). inv H1.
     Focus 3. intros ? ? H. inv H. reflexivity.
     replace i1 with (i1+0) by omega.
-    eapply (loop_merge (p:= fun c => halt (projT1 pM) (cstate c))). unfold halt at 2. cbn. 
+    eapply (loop_merge (p:= fun c => halt (projT1 pM) (cstate c))). unfold halt at 2. cbn.
     now intros ? ->. exact H'.
     apply loop_fulfills_p_0. unfold halt. cbn. rewrite px1.
     apply loop_fulfills_p in H'. now destruct halt.
     intros ? ? H ?. inv H. all: auto.
-    cbn in H0. f_equal. unfold step at 2;cbn. rewrite H0. now rewrite andb_false_r.
+    cbn in H0. f_equal. unfold step at 2;cbn. now rewrite H0.
   Qed.
 
 
-  Definition While_Rel (R : Rel (tapes sig n) (bool * F * tapes sig n)) :=
-    star (⋃_f R |_ (true, f)) ∘ R |_fst=false.
+  Variable R : pRel sig (option F) n.
+
+  Definition While_Rel : pRel sig F n := star (R |_ None) ∘ (fun (t : tapes sig n) '(y,t') => R t (Some y,t')).
 
 
-  Lemma While_Realise R :
-    pM ⊨ R -> WHILE ⊨ While_Rel R.
+  Lemma While_Realise :
+    pM ⊨ R -> WHILE ⊨ While_Rel.
   Proof.
     unfold While_Rel.
     intros HR t1 i1 oenc2 eq. unfold initc in eq.
@@ -124,26 +141,23 @@ Section While.
     {
       eapply loop_fulfills_p in Eq2. destruct halt; auto.
     }
-    apply andb_true_iff in Hoenc2 as (Hoenc2&Hoenc2'). apply negb_true_iff in Hoenc2'.
-    destruct (projT2 pM (cstate oenc2)) as [b f] eqn:Eoenc2.
-    destruct b; cbn in Hoenc2'; auto; clear Hoenc2'.
-    destruct (projT2 pM (cstate x0)) as [bx0 fx0] eqn:px0.
-    destruct bx0.
+    apply andb_true_iff in Hoenc2 as (Hoenc2&Hoenc2').
+    destruct (projT2 pM (cstate oenc2)) as [ f | ] eqn:Eoenc2; inv Hoenc2'.
+    destruct (projT2 pM (cstate x0)) as [ fx0 | ] eqn:px0.
+    - hnf. exists t1. split; [now apply starR | ]. hnf.
+      unfold  loopM in Eq2. rewrite loop_fulfills_p_0 in Eq2; [ | cbn; now rewrite px0, hx0]. inv Eq2.
+      apply HR in Eq1. cbn in Eq1. cbn. rewrite px0. cbn. auto. rewrite px0 in Eq1. auto.
     - eapply While_true_split in Eq2 as (i' & -> & Eq2); eauto.
       apply IH in Eq2; [ | omega]. hnf in Eq2.
       destruct Eq2 as (y&Eq2&Eq2'). hnf in Eq2, Eq2'.
       eapply use_subrel.
       rewrite <- star_rcomp_idem. rewrite rcomp_assoc. reflexivity.
       hnf. exists (ctapes x0). split.
-      + apply R_in_star. apply HR in Eq1. cbn in Eq1. rewrite px0 in Eq1. hnf. eauto.
+      + apply R_in_star. apply HR in Eq1. cbn in *. rewrite px0 in Eq1. rewrite Eoenc2 in Eq2'. eauto.
       + repeat (econstructor; hnf; eauto).
-    - hnf. exists t1. split; [now apply starR | ]. hnf.
-      unfold  loopM in Eq2. rewrite loop_fulfills_p_0 in Eq2; [ | cbn; now rewrite px0, hx0]. inv Eq2.
-      apply HR in Eq1. cbn in Eq1. cbn. rewrite px0. cbn. auto. rewrite px0 in Eq1. auto.
   Qed.
 
   Section While_terminatesIn.
-    Variable (R : Rel (tapes sig n) (bool * F * tapes sig n)).
     Variable (T T' : Rel (tapes sig n) nat).
 
     Lemma While_TerminatesIn :
@@ -153,27 +167,26 @@ Section While.
           T' tin i ->
           exists i1,
             T tin i1 /\
-            forall b yout tout,
-              R tin (b, yout, tout) ->
-              if b
-              then exists i2, T' tout i2 /\ 1 + i1 + i2 <= i
-              else i1 <= i) ->
-      While ↓(T').
+            forall (ymid : option F) tmid,
+              R tin (ymid, tmid) ->
+              match ymid with
+              | Some _ => i1 <= i
+              | None => exists i2, T' tmid i2 /\ 1 + i1 + i2 <= i
+              end) ->
+      While ↓T'.
     Proof.
       intros Realise_M Term_M Hyp tin i. revert tin. apply complete_induction with (x:=i); clear i; intros i IH tin.
       intros HT1. specialize (Hyp _ _ HT1) as (i1&Ht1&HT2).
       pose proof (Term_M _ _ Ht1) as (oconf&Hloop).
       specialize (Realise_M _ _ _ Hloop).
-      specialize (HT2 (fst (projT2 pM (cstate oconf))) (snd (projT2 pM (cstate oconf))) (ctapes oconf)).
-      rewrite <- surjective_pairing in HT2. specialize (HT2 Realise_M).
-      destruct (projT2 pM (cstate oconf)) as [bout yout] eqn:E1.
-      destruct bout; cbn in *.
-      - destruct HT2 as (i2&HT2&Hi).
-        specialize (IH i2 ltac:(omega) _ HT2) as (oconf2&Hloop2).
-        exists oconf2. eapply loop_ge with (k1 := i1 + (1 + i2)). omega.
-        eapply While_true_merge; eauto.
+      specialize (HT2 (projT2 pM (cstate oconf)) (ctapes oconf) Realise_M).
+      destruct (projT2 pM (cstate oconf)) as [ ymid | ] eqn:E1.
       - exists oconf. eapply loop_ge with (k1 := i1); eauto.
         eapply While_false_merge; eauto.
+      - destruct HT2 as (i2&HT2&Hi).
+        specialize (IH i2 ltac:(omega) _ HT2) as (oconf2&Hloop2).
+        exists oconf2. apply loop_ge with (k1 := i1 + (1 + i2)). omega.
+        eapply While_true_merge; eauto.
     Qed.
 
   End While_terminatesIn.
@@ -183,28 +196,27 @@ End While.
 
 Arguments While_Rel {n sig F} R x y/.
 Arguments WHILE : simpl never.
+Arguments WHILE {n sig F} pM {defF}.
 
 
 Section WhileInduction.
 
   Variable (sig : finType) (n : nat) (F : finType).
 
-  Variable R1 : Rel (tapes sig n) ((bool * F) * tapes sig n).
+  Variable R1 : Rel (tapes sig n) (option F * tapes sig n).
   Variable R2 : Rel (tapes sig n) (F * tapes sig n).
 
   Lemma WhileInduction :
-    (forall tin yout tout (HLastStep: (R1 |_fst=false) tin (yout, tout)), R2 tin (yout, tout)) ->
-    (forall tin tmid ymid tout yout
-       (HStar : (R1 |_(true, ymid)) tin tmid) (HLastStep : R2 tmid (yout, tout)), R2 tin (yout, tout)) ->
+    (forall tin yout tout (HLastStep: (R1 |_(Some yout)) tin tout), R2 tin (yout, tout)) ->
+    (forall tin tmid tout yout
+       (HStar : (R1 |_None) tin tmid) (HLastStep : R2 tmid (yout, tout)), R2 tin (yout, tout)) ->
     While_Rel R1 <<=2 R2.
   Proof.
     unfold While_Rel.
     intros H1 H2. intros tin (yout, tout) H.  cbn in H. destruct H as (tmid&HStar&HLastStep).
     induction HStar as [ tin | tin tmid tmid2 HS1 HS2 IH].
     - apply H1. cbn. apply HLastStep.
-    - cbn in HS1. destruct HS1 as (ymid, HS1). eapply H2.
-      + cbn. eapply HS1.
-      + apply IH. apply HLastStep.
+    - cbn in HS1. eauto.
   Qed.
 
 End WhileInduction.
